inference-tool/src/main/scala/inference/PrettyPrinting.scala
@@ -198,7 +198,7 @@ object PrettyPrinter {
     val pairs = r.map {
       case (k: Nat.nat, v: Option[Value.value]) =>
         s""""r${show(k)}":""" + (v match {
-          case None => throw new IllegalStateException("Got None from registers")
+          case None => "null"
           case Some(Value.Numa(Int.int_of_integer(n))) => n.toString
           case Some(Value.Str(s)) => s""""$s""""
         })
